
\documentclass[11pt]{article}

\usepackage{amsmath}
\usepackage{amsthm}
\usepackage{slashed}

\title{radix-4 Cooley-Tukey}
\author{Fedor Indutny}

\begin{document}

\maketitle

\begin{equation}
\begin{split}
X_k & = \sum^{N-1}_{n=0} x_n e^{-\frac{2 \pi i}{N} nk} \\
  & = \sum^{N/4 - 1}_{n=0} x_{4n} e^{-\frac{2 \pi i}{N/4} nk} + \
       x_{4n+1} e^{-\frac{2 \pi i}{N/4} (n+1/4) k} + \
       x_{4n+2} e^{-\frac{2 \pi i}{N/4} (n+2/4) k} + \\
  & \ \ \ \ \ \ \ \ x_{4n+3} e^{-\frac{2 \pi i}{N/4} (n+3/4) k} \\
  & = \sum^{N/4 - 1}_{n=0} x_{4n} e^{-\frac{2 \pi i}{N/4} nk} + \
        e^{-\frac{2 \pi i}{N}k} \sum^{N/4 - 1}_{n=0} x_{4n + 1} \
          e^{-\frac{2 \pi i}{N} nk} + \
        \dots \\
  & = A_k + e^{-\frac{2 \pi i}{N}k} B_k + \
        e^{-2 \frac{2 \pi i}{N}k} C_k + e^{-3 \frac{2 \pi i}{N}k} D_k
\end{split}
\end{equation}

Now, for $0 <= k < N/4$:

\begin{equation}
\begin{split}
X_{k + N/4} & = A_k + e^{-\frac{2 \pi i}{N}(k + N/4)} B_k + \
        e^{-2 \frac{2 \pi i}{N}(k + N/4)} C_k + e^{-3 \frac{2 \pi i}{N}(k+ N/4)} D_k \\
   & = A_k + e^{-\frac{1}{2} \pi i} e^{-\frac{2 \pi i}{N}k} B_k + \
         e^{-\pi i} e^{-2 \frac{2 \pi i}{N}k} C_k + \
         e^{-\frac{3}{2} \pi i} e^{-3 \frac{2 \pi i}{N}k} D_k \\
   & = A_k - i e^{-\frac{2 \pi i}{N}k} B_k - e^{-2 \frac{2 \pi i}{N}k} C_k + 
         i e^{-3 \frac{2 \pi i}{N}k} D_k
\end{split}
\end{equation}

So putting all together:

\begin{equation}
\begin{split}
X_k & = A_k + e^{-\frac{2 \pi i}{N}k} B_k + \
        e^{-2 \frac{2 \pi i}{N}k} C_k + e^{-3 \frac{2 \pi i}{N}k} D_k \\
X_{k + N/4} & = A_k - i e^{-\frac{2 \pi i}{N}k} B_k - e^{-2 \frac{2 \pi i}{N}k} C_k + \
         i e^{-3 \frac{2 \pi i}{N}k} D_k \\
X_{k + 2N/4} & = A_k - e^{-\frac{2 \pi i}{N}k} B_k + e^{-2 \frac{2 \pi i}{N}k} C_k \
  -e^{-3 \frac{2 \pi i}{N}k} D_k \\
X_{k + 3N/4} & = A_k + i e^{-\frac{2 \pi i}{N}k} B_k - e^{-2 \frac{2 \pi i}{N}k} C_k \
  -i e^{-3 \frac{2 \pi i}{N}k} D_k
\end{split}
\end{equation}

\end{document}